KB5_S5

Foundation/Modal/Hilbert/Geach.lean
@@ -31,6 +31,8 @@ instance K5.is_geach : (Hilbert.K5 α).IsGeach [⟨1, 1, 0, 1⟩] := by simp;
 
 instance KB4.is_geach : (Hilbert.KB4 α).IsGeach [⟨0, 1, 0, 1⟩, ⟨0, 2, 1, 0⟩] := by simp;
 
+instance KB5.is_geach : (Hilbert.KB5 α).IsGeach [⟨0, 1, 0, 1⟩, ⟨1, 1, 0, 1⟩] := by simp;
+
 instance KD.is_geach : (Hilbert.KD α).IsGeach [⟨0, 0, 1, 1⟩] := by simp;
 
 instance KD4.is_geach : (Hilbert.KD4 α).IsGeach [⟨0, 0, 1, 1⟩, ⟨0, 2, 1, 0⟩] := by simp;
